CDCLcm: instantiate locale

Weidenbach_Book/CDCL_W_Covering_Models.thy
@@ -4,17 +4,303 @@ begin
 
 section \<open>Covering Models\<close>
 
+text \<open>I am only interested in the extension of CDCL to find covering mdoels, not in the required
+subsequent extraction of the minimal covering models.\<close>
+
+type_synonym 'v cov = \<open>'v literal multiset multiset\<close>
+
 locale covering_models =
   fixes
     \<rho> :: \<open>'v \<Rightarrow> bool\<close>
 begin
-text \<open>
-  The first version of the calculus is probably wrong, because there is no totality
-  condition in the rule ConflCM.\<close>
 
-definition model_is_dominating :: \<open>'v literal multiset \<Rightarrow> 'v literal multiset \<Rightarrow> bool\<close> where
-\<open>model_is_dominating M M' \<longleftrightarrow>
+definition model_is_dominated :: \<open>'v literal multiset \<Rightarrow> 'v literal multiset \<Rightarrow> bool\<close> where
+\<open>model_is_dominated M M' \<longleftrightarrow>
   filter_mset (\<lambda>L. is_pos L \<and> \<rho> (atm_of L)) M \<subseteq># filter_mset (\<lambda>L. is_pos L \<and> \<rho> (atm_of L)) M'\<close>
+
+definition is_improving_int :: \<open>('v, 'v clause) ann_lits \<Rightarrow> ('v, 'v clause) ann_lits \<Rightarrow> 'v clauses \<Rightarrow> 'v cov \<Rightarrow> bool\<close> where
+\<open>is_improving_int M M' N \<M> \<longleftrightarrow>
+  (M = M' \<and> (\<forall>I \<in># \<M>. \<not>model_is_dominated (lit_of `# mset M) I)) \<and>
+  total_over_m (lits_of_l M) (set_mset N) \<and>
+  lit_of `# mset M \<in> simple_clss (atms_of_mm N) \<and>
+  M \<Turnstile>asm N \<and>
+  no_dup M\<close>
+
+
+text \<open>This criteria is a bit more general than Weidenbach's version.\<close>
+definition conflicting_clauses
+  :: \<open>'v clauses \<Rightarrow> 'v cov \<Rightarrow> 'v clauses\<close>
+where
+  \<open>conflicting_clauses N w =
+    {#C \<in># mset_set (simple_clss (atms_of_mm N)). pNeg `# w \<Turnstile>pm C#}\<close>
+
+lemma pNeg_simple_clss_iff[simp]:
+  \<open>pNeg M \<in> simple_clss N \<longleftrightarrow> M \<in> simple_clss N\<close>
+  by (auto simp: simple_clss_def)
+
+lemma conflicting_clauses_insert:
+  assumes \<open>M \<in> simple_clss (atms_of_mm N)\<close>
+  shows \<open>pNeg M \<in># conflicting_clauses N (add_mset M w)\<close>
+  using assms by (auto simp: conflicting_clauses_def simple_clss_finite)
+
+end
+
+locale conflict_driven_clause_learning\<^sub>W_covering_models =
+  conflict_driven_clause_learning\<^sub>W
+    state_eq
+    state
+    \<comment> \<open>functions for the state:\<close>
+      \<comment> \<open>access functions:\<close>
+    trail init_clss learned_clss conflicting
+      \<comment> \<open>changing state:\<close>
+    cons_trail tl_trail add_learned_cls remove_cls
+    update_conflicting
+      \<comment> \<open>get state:\<close>
+    init_state +
+  covering_models \<rho>
+  for
+    state_eq :: "'st \<Rightarrow> 'st \<Rightarrow> bool" (infix "\<sim>" 50) and
+    state :: "'st \<Rightarrow> ('v, 'v clause) ann_lits \<times> 'v clauses \<times> 'v clauses \<times> 'v clause option \<times>
+      'v cov \<times> 'b" and
+    trail :: "'st \<Rightarrow> ('v, 'v clause) ann_lits" and
+    init_clss :: "'st \<Rightarrow> 'v clauses" and
+    learned_clss :: "'st \<Rightarrow> 'v clauses" and
+    conflicting :: "'st \<Rightarrow> 'v clause option" and
+
+    cons_trail :: "('v, 'v clause) ann_lit \<Rightarrow> 'st \<Rightarrow> 'st" and
+    tl_trail :: "'st \<Rightarrow> 'st" and
+    add_learned_cls :: "'v clause \<Rightarrow> 'st \<Rightarrow> 'st" and
+    remove_cls :: "'v clause \<Rightarrow> 'st \<Rightarrow> 'st" and
+    update_conflicting :: "'v clause option \<Rightarrow> 'st \<Rightarrow> 'st" and
+    init_state :: "'v clauses \<Rightarrow> 'st" and
+    \<rho> :: \<open>'v \<Rightarrow> bool\<close>  +
+  fixes
+    update_additional_info :: \<open>'v cov \<times> 'b \<Rightarrow> 'st \<Rightarrow> 'st\<close>
+  assumes
+    update_additional_info:
+      \<open>state S = (M, N, U, C, \<M>) \<Longrightarrow> state (update_additional_info K' S) = (M, N, U, C, K')\<close> and
+    weight_init_state:
+      \<open>\<And>N :: 'v clauses. fst (additional_info (init_state N)) = {#}\<close>
+begin
+
+definition update_weight_information :: \<open>('v, 'v clause) ann_lits \<Rightarrow> 'st \<Rightarrow> 'st\<close> where
+  \<open>update_weight_information M S =
+    update_additional_info (add_mset (lit_of `# mset M) (fst (additional_info S)), snd (additional_info S)) S\<close>
+
+lemma
+  trail_update_additional_info[simp]: \<open>trail (update_additional_info w S) = trail S\<close> and
+  init_clss_update_additional_info[simp]:
+    \<open>init_clss (update_additional_info w S) = init_clss S\<close> and
+  learned_clss_update_additional_info[simp]:
+    \<open>learned_clss (update_additional_info w S) = learned_clss S\<close> and
+  backtrack_lvl_update_additional_info[simp]:
+    \<open>backtrack_lvl (update_additional_info w S) = backtrack_lvl S\<close> and
+  conflicting_update_additional_info[simp]:
+    \<open>conflicting (update_additional_info w S) = conflicting S\<close> and
+  clauses_update_additional_info[simp]:
+    \<open>clauses (update_additional_info w S) = clauses S\<close>
+  using update_additional_info[of S] unfolding clauses_def
+  by (subst (asm) state_prop; subst (asm) state_prop; auto; fail)+
+
+lemma
+  trail_update_weight_information[simp]:
+    \<open>trail (update_weight_information w S) = trail S\<close> and
+  init_clss_update_weight_information[simp]:
+    \<open>init_clss (update_weight_information w S) = init_clss S\<close> and
+  learned_clss_update_weight_information[simp]:
+    \<open>learned_clss (update_weight_information w S) = learned_clss S\<close> and
+  backtrack_lvl_update_weight_information[simp]:
+    \<open>backtrack_lvl (update_weight_information w S) = backtrack_lvl S\<close> and
+  conflicting_update_weight_information[simp]:
+    \<open>conflicting (update_weight_information w S) = conflicting S\<close> and
+  clauses_update_weight_information[simp]:
+    \<open>clauses (update_weight_information w S) = clauses S\<close>
+  using update_additional_info[of S] unfolding update_weight_information_def by auto
+
+definition covering :: \<open>'st \<Rightarrow> 'v cov\<close> where
+  \<open>covering S = fst (additional_info S)\<close>
+
+lemma
+  additional_info_update_additional_info[simp]:
+  "additional_info (update_additional_info w S) = w"
+  unfolding additional_info_def using update_additional_info[of S]
+  by (cases \<open>state S\<close>; auto; fail)+
+
+lemma
+  covering_cons_trail2[simp]: \<open>covering (cons_trail L S) = covering S\<close> and
+  clss_tl_trail2[simp]: "covering (tl_trail S) = covering S" and
+  covering_add_learned_cls_unfolded:
+    "covering (add_learned_cls U S) = covering S"
+    and
+  covering_update_conflicting2[simp]: "covering (update_conflicting D S) = covering S" and
+  covering_remove_cls2[simp]:
+    "covering (remove_cls C S) = covering S" and
+  covering_add_learned_cls2[simp]:
+    "covering (add_learned_cls C S) = covering S" and
+  covering_update_covering_information2[simp]:
+    "covering (update_weight_information M S) = add_mset (lit_of `# mset M) (covering S)"
+  by (auto simp: update_weight_information_def covering_def)
+
+
+
+sublocale conflict_driven_clause_learning\<^sub>W where
+  state_eq = state_eq and
+  state = state and
+  trail = trail and
+  init_clss = init_clss and
+  learned_clss = learned_clss and
+  conflicting = conflicting and
+  cons_trail = cons_trail and
+  tl_trail = tl_trail and
+  add_learned_cls = add_learned_cls and
+  remove_cls = remove_cls and
+  update_conflicting = update_conflicting and
+  init_state = init_state
+  by unfold_locales
+
+sublocale conflict_driven_clause_learning_with_adding_init_clause_cost\<^sub>W_no_state
+  where
+    state = state and
+    trail = trail and
+    init_clss = init_clss and
+    learned_clss = learned_clss and
+    conflicting = conflicting and
+    cons_trail = cons_trail and
+    tl_trail = tl_trail and
+    add_learned_cls = add_learned_cls and
+    remove_cls = remove_cls and
+    update_conflicting = update_conflicting and
+    init_state = init_state and
+    weight = covering and
+    update_weight_information = update_weight_information and
+    is_improving_int = is_improving_int and
+    conflicting_clauses = conflicting_clauses
+  by unfold_locales
+
+lemma state_additional_info2':
+  \<open>state S = (trail S, init_clss S, learned_clss S, conflicting S, covering S, additional_info' S)\<close>
+  unfolding additional_info'_def by (cases \<open>state S\<close>; auto simp: state_prop covering_def)
+
+lemma state_update_weight_information:
+  \<open>state S = (M, N, U, C, w, other) \<Longrightarrow>
+    \<exists>w'. state (update_weight_information T S) = (M, N, U, C, w', other)\<close>
+  unfolding update_weight_information_def by (cases \<open>state S\<close>; auto simp: state_prop covering_def)
+
+
+lemma conflicting_clss_incl_init_clss:
+  \<open>atms_of_mm (conflicting_clss S) \<subseteq> atms_of_mm (init_clss S)\<close>
+  unfolding conflicting_clss_def conflicting_clauses_def
+  apply (auto simp: simple_clss_finite)
+  by (auto simp: simple_clss_def atms_of_ms_def split: if_splits)
+
+lemma conflict_clss_update_weight_no_alien:
+  \<open>atms_of_mm (conflicting_clss (update_weight_information M S))
+    \<subseteq> atms_of_mm (init_clss S)\<close>
+  by (auto simp: conflicting_clss_def conflicting_clauses_def atms_of_ms_def
+      cdcl\<^sub>W_restart_mset_state simple_clss_finite
+    dest: simple_clssE)
+
+
+lemma distinct_mset_mset_conflicting_clss2: \<open>distinct_mset_mset (conflicting_clss S)\<close>
+  unfolding conflicting_clss_def conflicting_clauses_def distinct_mset_set_def
+  apply (auto simp: simple_clss_finite)
+  by (auto simp: simple_clss_def)
+
+
+lemma total_over_m_atms_incl:
+  assumes \<open>total_over_m M (set_mset N)\<close>
+  shows
+    \<open>x \<in> atms_of_mm N \<Longrightarrow> x \<in> atms_of_s M\<close>
+  by (meson assms contra_subsetD total_over_m_alt_def)
+
+lemma conflicting_clss_update_weight_information_in2:
+  assumes \<open>is_improving M M' S\<close>
+  shows \<open>negate_ann_lits M' \<in># conflicting_clss (update_weight_information M' S)\<close>
+  using assms apply (auto simp: simple_clss_finite
+    conflicting_clauses_def conflicting_clss_def is_improving_int_def)
+  by (auto simp: is_improving_int_def conflicting_clss_def conflicting_clauses_def
+      simp: multiset_filter_mono2 simple_clss_def lits_of_def
+      negate_ann_lits_pNeg_lit_of image_iff dest: total_over_m_atms_incl
+      intro!: true_clss_cls_in)
+
+lemma is_improving_conflicting_clss_update_weight_information: \<open>is_improving M M' S \<Longrightarrow>
+       conflicting_clss S \<subseteq># conflicting_clss (update_weight_information M' S)\<close>
+  by (auto simp: is_improving_int_def conflicting_clss_def conflicting_clauses_def
+      simp: multiset_filter_mono2 le_less true_clss_cls_tautology_iff simple_clss_finite
+      intro!: image_mset_subseteq_mono
+      dest: simple_clssE
+      split: enat.splits)
+
+sublocale state\<^sub>W_no_state
+  where
+    state = state and
+    trail = trail and
+    init_clss = init_clss and
+    learned_clss = learned_clss and
+    conflicting = conflicting and
+    cons_trail = cons_trail and
+    tl_trail = tl_trail and
+    add_learned_cls = add_learned_cls and
+    remove_cls = remove_cls and
+    update_conflicting = update_conflicting and
+    init_state = init_state
+  by unfold_locales
+
+sublocale state\<^sub>W_no_state where
+  state_eq = state_eq and
+  state = state and
+  trail = trail and
+  init_clss = init_clss and
+  learned_clss = learned_clss and
+  conflicting = conflicting and
+  cons_trail = cons_trail and
+  tl_trail = tl_trail and
+  add_learned_cls = add_learned_cls and
+  remove_cls = remove_cls and
+  update_conflicting = update_conflicting and
+  init_state = init_state
+  by unfold_locales
+
+sublocale conflict_driven_clause_learning\<^sub>W where
+  state_eq = state_eq and
+  state = state and
+  trail = trail and
+  init_clss = init_clss and
+  learned_clss = learned_clss and
+  conflicting = conflicting and
+  cons_trail = cons_trail and
+  tl_trail = tl_trail and
+  add_learned_cls = add_learned_cls and
+  remove_cls = remove_cls and
+  update_conflicting = update_conflicting and
+  init_state = init_state
+  by unfold_locales
+
+sublocale conflict_driven_clause_learning_with_adding_init_clause_cost\<^sub>W_ops
+  where
+    state = state and
+    trail = trail and
+    init_clss = init_clss and
+    learned_clss = learned_clss and
+    conflicting = conflicting and
+    cons_trail = cons_trail and
+    tl_trail = tl_trail and
+    add_learned_cls = add_learned_cls and
+    remove_cls = remove_cls and
+    update_conflicting = update_conflicting and
+    init_state = init_state and
+    weight = covering and
+    update_weight_information = update_weight_information and
+    is_improving_int = is_improving_int and
+    conflicting_clauses = conflicting_clauses
+  apply unfold_locales
+  subgoal by (rule state_additional_info2')
+  subgoal by (rule state_update_weight_information)
+  subgoal by (rule conflicting_clss_incl_init_clss)
+  subgoal by (rule distinct_mset_mset_conflicting_clss2)
+  subgoal by (rule is_improving_conflicting_clss_update_weight_information)
+  subgoal by (rule conflicting_clss_update_weight_information_in2)
+  done
 
 end
 
